treesort

lectures/src/treesort.v
@@ -23,17 +23,18 @@ Fixpoint root (A : Set)(default : A)(t : Tree A) : A :=
   | node l a r => a
   end.
 
-Fixpoint Everywhere (A : Set)(P : A -> Prop)(t : Tree A) {struct t} 
+Fixpoint EverywhereT (A : Set)(P : A -> Prop)(t : Tree A) {struct t} 
   : Prop :=
   match t with
   | leaf => True
-  | node l a r => Everywhere P l /\ P a /\ Everywhere P r
+  | node l a r => EverywhereT P l /\ P a /\ EverywhereT P r
   end.
 
 Fixpoint SortedTree (t : Tree nat) : Prop :=
   match t with
   | leaf => True
-  | node l a r => root a l <= a /\ a <= root a r 
+  | node l a r => EverywhereT (fun x => x <= a) l
+               /\ EverywhereT (fun x => a <= x) r
                /\ SortedTree l /\ SortedTree r
   end.
 
@@ -65,55 +66,66 @@ Eval compute in tsort (4::2::3::1::nil).
 Axiom CaseInsertT : forall (t : Tree nat)(n d : nat),
   root d (insertT n t) = n \/ root d (insertT n t) = root d t.
 
+Lemma insertTeverywhere : 
+  forall (P : nat -> Prop)(n : nat)(t : Tree nat),
+    P n -> EverywhereT P t -> EverywhereT P (insertT n t).
+intros P n t p.
+induction t.
+intro h.
+simpl.
+split. split. split. exact p. split.
+intro h.
+simpl in h.
+destruct h as [et1 h]. destruct h as [pa et2].
+simpl.
+destruct (leqb n a).
+simpl.
+split.
+apply IHt1.
+exact et1.
+split.
+exact pa.
+exact et2.
+simpl.
+split.
+exact et1.
+split.
+exact pa.
+apply IHt2.
+exact et2.
+Qed.
+
+
 Lemma insertTSorted : forall (t : Tree nat)(n : nat),
   SortedTree t -> SortedTree (insertT n t).
 intros t n.
 induction t.
 intro h.
 simpl.
-split.
-apply le_refl.
-split.
-apply le_refl.
-split. split. split.
+split. split. split. split. split. split. split.
 intro h.
-simpl.
 simpl in h.
-destruct h as [t1a h].
-destruct h as [at2 h].
+destruct h as [et1 h]. destruct h as [et2 h].
 destruct h as [st1 st2].
+simpl.
 case_eq (leqb n a).
 intro na.
 simpl.
 split.
-destruct (CaseInsertT t1 n a) as [h1 | h2].
-rewrite h1.
-apply leq1.
-exact na.
-rewrite h2.
-exact t1a.
-split.
-exact at2.
-split.
-apply IHt1.
-exact st1.
+apply insertTeverywhere.
+apply leq1. exact na.
+exact et1.
+split. exact et2.
+split. apply IHt1. exact st1.
 exact st2.
 intro an.
-simpl.
-split.
-exact t1a.
-split.
-destruct (CaseInsertT t2 n a) as [h1 | h2].
-rewrite h1.
-apply leqFalse.
-exact an.
-rewrite h2.
-exact at2.
-split.
-exact st1.
-apply IHt2.
-exact st2.
+simpl. split. apply et1.
+split. apply insertTeverywhere.
+apply leqFalse. exact an.
+exact et2.
+split. exact st1. apply IHt2. exact st2.
 Qed.
+
 
 Lemma buildTreeSorted : forall ns : list nat, SortedTree (buildTree ns).
 intro ns.
@@ -124,6 +136,36 @@ simpl.
 apply insertTSorted.
 exact IHns.
 Qed.
+
+Fixpoint EverywhereL (A : Set)(P : A -> Prop)(l : list A) {struct l}
+  : Prop :=
+  match l with
+  | nil => True
+  | a :: l => P a /\ EverywhereL P l
+  end.
+
+Axiom everywhereDestruct : 
+  forall (P : nat -> Prop)(t : Tree nat),
+    EverywhereT P t -> EverywhereL P (destructTree t).
+
+Lemma sortAppLem : forall (l1 l2 : list nat)(n : nat),
+  Sorted l1 -> Sorted (n::l2) -> EverywhereL (fun x => x <= n) l1
+  -> Sorted (l1 ++ n :: l2).
+induction l1.
+intros. exact H0.
+intros.
+simpl.
+simpl in H1.
+destruct H1 as [an el1].
+split.
+apply IHl1.
+simpl in H.
+destruct H as [sl1 al1].
+exact sl1.
+exact H0.
+exact el1.
+
+
 
 Lemma destructTreeSorted : forall ns : Tree nat, 
   SortedTree ns -> Sorted (destructTree ns).
